gravy/test/out.bpl
@@ -11,21 +11,6 @@ const unique $type : Field javaType;
 const unique $alloc : Field bool;
 const { :sourceloc "Object.java",-1,-1,-1,-1 } unique java.lang.Object : javaType extends  complete;
 const { :sourceloc "InfeasibleCode01.java",-1,-1,-1,-1 } unique InfeasibleCode01 : javaType extends  unique java.lang.Object complete;
-const { :sourceloc "Appendable.java",-1,-1,-1,-1 } unique java.lang.Appendable : javaType extends  unique java.lang.Object complete;
-const { :sourceloc "CharSequence.java",-1,-1,-1,-1 } unique java.lang.CharSequence : javaType extends  unique java.lang.Object complete;
-const { :sourceloc "AbstractStringBuilder.java",-1,-1,-1,-1 } unique java.lang.AbstractStringBuilder : javaType extends  unique java.lang.Object, unique java.lang.Appendable, unique java.lang.CharSequence complete;
-const { :sourceloc "Serializable.java",-1,-1,-1,-1 } unique java.io.Serializable : javaType extends  unique java.lang.Object complete;
-const { :sourceloc "StringBuffer.java",-1,-1,-1,-1 } unique java.lang.StringBuffer : javaType extends  unique java.io.Serializable, unique java.lang.AbstractStringBuilder, unique java.lang.CharSequence complete;
-const { :sourceloc "Comparable.java",-1,-1,-1,-1 } unique java.lang.Comparable : javaType extends  unique java.lang.Object complete;
-const { :sourceloc "String.java",-1,-1,-1,-1 } unique java.lang.String : javaType extends  unique java.io.Serializable, unique java.lang.Object, unique java.lang.Comparable, unique java.lang.CharSequence complete;
-const unique $StringConst0 : ref extends  complete;
-const { :sourceloc "AutoCloseable.java",-1,-1,-1,-1 } unique java.lang.AutoCloseable : javaType extends  unique java.lang.Object complete;
-const { :sourceloc "Closeable.java",-1,-1,-1,-1 } unique java.io.Closeable : javaType extends  unique java.lang.AutoCloseable, unique java.lang.Object complete;
-const { :sourceloc "Flushable.java",-1,-1,-1,-1 } unique java.io.Flushable : javaType extends  unique java.lang.Object complete;
-const { :sourceloc "OutputStream.java",-1,-1,-1,-1 } unique java.io.OutputStream : javaType extends  unique java.lang.Object, unique java.io.Closeable, unique java.io.Flushable complete;
-const { :sourceloc "FilterOutputStream.java",-1,-1,-1,-1 } unique java.io.FilterOutputStream : javaType extends  unique java.io.OutputStream complete;
-const { :sourceloc "PrintStream.java",-1,-1,-1,-1 } unique java.io.PrintStream : javaType extends  unique java.io.Closeable, unique java.lang.Appendable, unique java.io.FilterOutputStream complete;
-const unique $StringConst1 : ref extends  complete;
 var $heap : $heap_type;
 var $intArrayType : javaType;
 var $charArrayType : javaType;
@@ -38,7 +23,6 @@ var $boolArrHeap : boolArrHeap_type;
 var $refArrHeap : refArrHeap_type;
 var $realArrHeap : realArrHeap_type;
 var $intArrHeap : intArrHeap_type;
-var java.io.PrintStream$java.lang.System$err236 : ref;
 function $arrayType(t:javaType) returns ($ret:javaType);
 function $intToReal(x:int) returns ($ret:real);
 function $intToBool(x:int) returns ($ret:bool) { (if x == 0 then false else true) }
@@ -54,79 +38,94 @@ function $xorInt(x:int, y:int) returns ($ret:int);
 function $shlInt(x:int, y:int) returns ($ret:int);
 function $ushrInt(x:int, y:int) returns ($ret:int);
 function $shrInt(x:int, y:int) returns ($ret:int);
-procedure $new(obj_type:javaType) returns ($obj:ref);        requires $heap[$obj,$alloc] == false;    ensures $heap[$obj,$alloc] == true;    ensures $obj != $null;    ensures $heap[$obj,$type] == obj_type;
+procedure $new(obj_type:javaType) returns ($obj:ref);    ensures $obj != $null;        ensures $heap[$obj,$type] == obj_type;    requires $heap[$obj,$alloc] == false;    ensures $heap[$obj,$alloc] == true;
 
-procedure java.lang.Object$java.lang.Object$clone$43($this:ref) returns ($other:ref);        ensures $heap[$other,$alloc] == true;    ensures $other != $null;    ensures $heap[$other,$type] == $heap[$this,$type];
+procedure java.lang.Object$java.lang.Object$clone$43($this:ref) returns ($other:ref);        ensures $other != $null;    ensures $heap[$other,$alloc] == true;    ensures $heap[$other,$type] == $heap[$this,$type];
 
-procedure int$java.lang.String$compareTo$87($this:ref, $other:ref) returns ($return:int);    ensures ($this == $other ==> $return == 1) && ($this != $other ==> $return == 0);    
+procedure int$java.lang.String$compareTo$87($this:ref, $other:ref) returns ($return:int);        ensures ($this == $other ==> $return == 1) && ($this != $other ==> $return == 0);
 
-procedure int$InfeasibleCode01$infeasible0$1889($this:ref, $in_parameter__0:ref) returns ($return:int, $exception:ref);    modifies $intArrHeap;
+procedure void$InfeasibleCode01$feasible01$1889($this:ref, $in_parameter__0:ref) returns ($exception:ref);    
 
-procedure int$InfeasibleCode01$infeasible1$1890($this:ref, $in_parameter__0:ref) returns ($return:int, $exception:ref);    
-
-procedure int$java.lang.Object$hashCode$41($this:ref) returns ($return:int, $exception:ref);    
-
-procedure void$java.lang.StringBuffer$$la$init$ra$$685($this:ref) returns ($exception:ref);    
-
-procedure java.lang.String$java.lang.Object$toString$44($this:ref) returns ($return:ref, $exception:ref);    
-
-procedure java.lang.StringBuffer$java.lang.StringBuffer$append$701($this:ref, $in_parameter__0:ref) returns ($return:ref, $exception:ref);    
-
-procedure java.lang.String$java.lang.StringBuffer$toString$738($this:ref) returns ($return:ref, $exception:ref);    
-
-procedure void$java.io.PrintStream$println$217($this:ref, $in_parameter__0:ref) returns ($exception:ref);    
-
-procedure void$InfeasibleCode01$infeasible2$1891($this:ref, $in_parameter__0:ref) returns ($exception:ref);    modifies $intArrHeap;
-
-procedure void$InfeasibleCode01$infeasible3$1892($this:ref, $in_parameter__0:int, $in_parameter__1:int) returns ($exception:ref);    
-
-procedure boolean$InfeasibleCode01$infeasible4$1893($this:ref, $in_parameter__0:ref) returns ($return:int, $exception:ref);    
-
-procedure void$InfeasibleCode01$infeasible5$1894($this:ref) returns ($exception:ref);    modifies $stringSizeHeap;
-
-procedure int$InfeasibleCode01$infeasible6$1895($this:ref, $in_parameter__0:ref) returns ($return:int, $exception:ref);    
-
-procedure void$InfeasibleCode01$$la$init$ra$$1896($this:ref) returns ($exception:ref);    
+procedure void$InfeasibleCode01$$la$init$ra$$1890($this:ref) returns ($exception:ref);    
 
 procedure void$java.lang.Object$$la$init$ra$$38($this:ref) returns ($exception:ref);    
 
-implementation void$InfeasibleCode01$infeasible2$1891($this:ref, $in_parameter__0:ref) returns ($exception:ref){
+implementation void$InfeasibleCode01$feasible01$1889($this:ref, $in_parameter__0:ref) returns ($exception:ref){
     
-var temp$122 : ref;    
-var temp$021 : int;    
-var temp$324 : int;    
-var i20 : int;    
-var this18 : ref;    
-var arr19 : ref;    
-var temp$223 : int;    
-var temp$425 : int;
+var this1 : ref;    
+var temp$410 : int;    
+var temp2 : ref;    
+var temp$814 : int;    
+var temp$39 : int;    
+var j5 : int;    
+var temp$612 : int;    
+var temp$511 : int;    
+var temp$17 : int;    
+var repos3 : int;    
+var temp$06 : int;    
+var temp$28 : ref;    
+var temp$713 : int;    
+var end4 : int;    
+var temp$915 : int;
     assume $this != $null;
-    this18 := $this;
-    arr19 := $in_parameter__0;
-    i20 := 0;
+    this1 := $this;
+    temp2 := $in_parameter__0;
+    repos3 := -1;
+    end4 := -1;
+    assert { :sourceloc "InfeasibleCode01.java",76,3,76,22 } temp2 != $null;
+    j5 := $arrSizeHeap[temp2];
+    j5 := end4;
+  block1:
+    temp$06 := j5;
+    temp$17 := temp$06 + 1;
+    j5 := temp$17;
+    temp$28 := temp2;
+    temp$39 := j5;
+    assert { :sourceloc "InfeasibleCode01.java",86,8,86,19 } temp$39 < $arrSizeHeap[temp$28] && temp$39 >= 0;
+    temp$410 := $intArrHeap[temp$28][temp$39];
+    temp$511 := temp$410;
+    if (temp$511 == 97) {
+        assert { :sourceloc "InfeasibleCode01.java",86,8,86,19 } true;
+        goto block2;
+    } else {
+        assert { :sourceloc "InfeasibleCode01.java",86,8,86,19 } true;
+    }
+    goto block3;
+  block2:
+    temp$612 := j5 - end4;
+    temp$713 := temp$612 - 1;
+    repos3 := temp$713;
   block3:
-    assert { :sourceloc "InfeasibleCode01.java",42,17,42,29 } arr19 != $null;
-    temp$021 := $arrSizeHeap[arr19];
-    if (i20 <= temp$021) {
-        assert { :sourceloc "InfeasibleCode01.java",42,17,42,29 } true;
+    if (repos3 == -1) {
+        assert { :sourceloc "InfeasibleCode01.java",89,12,89,22 } true;
         goto block4;
     } else {
-        assert { :sourceloc "InfeasibleCode01.java",42,17,42,29 } true;
+        assert { :sourceloc "InfeasibleCode01.java",89,12,89,22 } true;
     }
     goto block5;
   block4:
-    temp$122 := arr19;
-    temp$223 := i20;
-    assert { :sourceloc "InfeasibleCode01.java",43,7,43,9 } temp$223 < $arrSizeHeap[temp$122] && temp$223 >= 0;
-    $intArrHeap := $intArrHeap[temp$122 := $intArrHeap[temp$122][temp$223 := i20]];
-    temp$324 := i20;
-    temp$425 := temp$324 + 1;
-    i20 := temp$425;
-    goto block3;
+    assert { :sourceloc "InfeasibleCode01.java",89,27,89,41 } temp2 != $null;
+    temp$814 := $arrSizeHeap[temp2];
+    if (j5 < temp$814) {
+        assert { :sourceloc "InfeasibleCode01.java",84,3,89,43 } true;
+        goto block1;
+    } else {
+        assert { :sourceloc "InfeasibleCode01.java",89,27,89,41 } true;
+    }
+    goto block5;
+    goto block1;
   block5:
-	assert { :sourceloc "InfeasibleCode01.java",100,17,100,29 } true;
+    if (repos3 == -1) {
+        assert { :sourceloc "InfeasibleCode01.java",90,7,90,17 } true;
+        goto block6;
+    } else {
+        assert { :sourceloc "InfeasibleCode01.java",90,7,90,17 } true;
+    }
+    goto block7;
+  block6:
+    temp$915 := 0;
+    repos3 := temp$915;
+  block7:
     return;
 }
-
-
 
